Logic/Predicate/Semantics.lean
@@ -1,52 +1,141 @@
 import Logic.Predicate.Term
 
-variable {L : Language} {μ μ₁ μ₂ : Type _}
+universe u u₁ u₂ v v₁ v₂ w w₁ w₂
 
-structure Structure₁ (L : Language.{u}) :=
-(dom : Type u)
-(domInhabited : Inhabited dom)
-(func : {k : ℕ} → L.func k → (Fin k → dom) → dom)
-(rel : {k : ℕ} → L.rel  k → (Fin k → dom) → Prop)
+variable
+  {L : Language.{u}} {L₁ : Language.{u₁}} {L₂ : Language.{u₂}}
+  {μ : Type v} {μ₁ : Type v₁} {μ₂ : Type v₂}
 
-instance Structure₁_coe : CoeSort (Structure₁ L) (Type _) := ⟨Structure₁.dom⟩
+@[ext] class Structure₁ (L : Language.{u}) (M : Type w) :=
+  (func : {k : ℕ} → L.func k → (Fin k → M) → M)
+  (rel : {k : ℕ} → L.rel  k → (Fin k → M) → Prop)
 
-instance Structure₁_Inhabited (S : Structure₁ L) : Inhabited S := S.domInhabited
+namespace Language
+namespace Hom
+
+/-
+set_option linter.unusedVariables false in
+def onModel₁ (Φ : L₁ →ᵥ L₂) (M₂ : Type w₂) [Structure₁ L₂ M₂] := M₂
+
+def cast (Φ : L₁ →ᵥ L₂) {M₂ : Type w₂} [Structure₁ L₂ M₂] (a : M₂) : Φ.onModel₁ M₂ := a
+
+def uncast (Φ : L₁ →ᵥ L₂) {M₂ : Type w₂} [Structure₁ L₂ M₂] (a : Φ.onModel₁ M₂) : M₂ := a
+
+variable {Φ : L₁ →ᵥ L₂} {M₂ : Type w₂} [Structure₁ L₂ M₂]
+
+instance [Inhabited M₂] : Inhabited (Φ.onModel₁ M₂) := ⟨Φ.cast default⟩
+
+@[simp] lemma uncast_cast (a : M₂) : Φ.uncast (Φ.cast a) = a := rfl
+
+@[simp] lemma cast_uncast (a : Φ.onModel₁ M₂) : Φ.cast (Φ.uncast a) = a := rfl
+
+lemma cast_injective : Function.Injective (Φ.cast : M₂ → Φ.onModel₁ M₂) := fun _ _ => id
+
+lemma uncast_injective : Function.Injective (Φ.uncast : Φ.onModel₁ M₂ → M₂) := fun _ _ => id
+
+@[simp] lemma cast_inj_iff (a b : M₂) : Φ.cast a = Φ.cast b ↔ a = b := cast_injective.eq_iff
+
+@[simp] lemma uncast_inj_iff (a b : Φ.onModel₁ M₂) : Φ.uncast a = Φ.uncast b ↔ a = b := uncast_injective.eq_iff
+
+attribute [irreducible] onModel₁
+-/
+
+def onStructure₁ (Φ : L₁ →ᵥ L₂) {M : Type w} (S : Structure₁ L₂ M) : Structure₁ L₁ M where
+  func := fun f => S.func (Φ.onFunc f)
+  rel := fun r => S.rel (Φ.onRel r)
+
+instance subLanguageStructure₁ {pfunc : ∀ k, Language.func L k → Prop} {prel : ∀ k, L.rel k → Prop}
+  {M : Type w} [s : Structure₁ L M] : Structure₁ (subLanguage L pfunc prel) M :=
+  onStructure₁ (ofSub L) s
+
+end Hom
+end Language
+
+namespace Structure₁
+
+instance [Inhabited M] : Inhabited (Structure₁ L M) :=
+⟨{ func := fun _ _ => default, rel := fun _ _ => True }⟩
+
+variable (Φ : L₁ →ᵥ L₂) {M : Type w} (S : Structure₁ L₂ M)
+
+/-
+instance [Structure₁ L₂ M₂] : Structure₁ L₁ (Φ.onModel₁ M₂) where
+  func := fun f v => Φ.cast $ Structure₁.func (Φ.onFunc f) (Φ.uncast ∘ v)
+  rel := fun r v => Structure₁.rel (Φ.onRel r) (Φ.uncast ∘ v)
+
+@[simp] lemma onModel₁_func {k} {f : L₁.func k} {v : Fin k → Φ.onModel₁ M₂} :
+    func f v = (Φ.cast $ func (Φ.onFunc f) (Φ.uncast ∘ v)) := rfl
+
+@[simp] lemma onModel₁_rel {k} {r : L₁.rel k} {v : Fin k → Φ.onModel₁ M₂} :
+    rel r v ↔ rel (Φ.onRel r) (Φ.uncast ∘ v) := of_eq rfl
+-/
+
+@[simp] lemma onStructure₁_func {k} {f : L₁.func k} {v : Fin k → M} :
+    (Φ.onStructure₁ S).func f v = S.func (Φ.onFunc f) v := rfl
+
+@[simp] lemma onStructure₁_rel {k} {r : L₁.rel k} {v : Fin k → M} :
+    (Φ.onStructure₁ S).rel r v ↔ S.rel (Φ.onRel r) v := of_eq rfl
+
+end Structure₁
 
 namespace SubTerm
-variable {n n₁ n₂ : ℕ} (S : Structure₁ L) (e : Fin n → S) (Φ : μ → S)
 
-@[simp] def val : SubTerm L μ n → S
-  | (#x)       => e x
-  | (&x)       => Φ x
-  | (func f v) => S.func f (fun i => (v i).val)
+variable {M} (s : Structure₁ L M) {n n₁ n₂ : ℕ} (e : Fin n → M) (e₂ : Fin n₂ → M) (ε : μ → M) (ε₂ : μ₂ → M)
 
-lemma val_bind (fixed : Fin n₁ → SubTerm L μ₂ n₂) (free : μ₁ → SubTerm L μ₂ n₂) (e : Fin n₂ → S) (Φ : μ₂ → S) (t : SubTerm L μ₁ n₁) :
-    (bind fixed free t).val S e Φ = t.val S (fun x => val S e Φ (fixed x)) (fun x => val S e Φ (free x)) :=
+def val : SubTerm L μ n → M
+  | #x       => e x
+  | &x       => ε x
+  | func f v => s.func f (fun i => (v i).val)
+
+variable (M) {s}
+
+@[reducible] def val! [s : Structure₁ L M] {n} (e : Fin n → M) (ε : μ → M) : SubTerm L μ n → M := val s e ε
+
+variable {M e e₂ ε ε₂}
+
+@[simp] lemma val_fixedVar (x) : val s e ε (#x : SubTerm L μ n) = e x := rfl
+
+@[simp] lemma val_freeVar (x) : val s e ε (&x : SubTerm L μ n) = ε x := rfl
+
+@[simp] lemma val_func {k} (f : L.func k) (v) :
+    val s e ε (func f v) = s.func f (fun i => (v i).val s e ε) := rfl
+  
+lemma val_bind (fixed : Fin n₁ → SubTerm L μ₂ n₂) (free : μ₁ → SubTerm L μ₂ n₂) (t : SubTerm L μ₁ n₁) :
+    (bind fixed free t).val s e₂ ε₂ = t.val s (val s e₂ ε₂ ∘ fixed) (val s e₂ ε₂ ∘ free) :=
   by induction t <;> simp[*]
 
-lemma val_map (fixed : Fin n₁ → Fin n₂) (free : μ₁ → μ₂) (e : Fin n₂ → S) (Φ : μ₂ → S) (t : SubTerm L μ₁ n₁) :
-    (map fixed free t).val S e Φ = t.val S (fun x => e (fixed x)) (fun x => Φ (free x)) := val_bind _ _ _ _ _ _
+lemma val_map (fixed : Fin n₁ → Fin n₂) (free : μ₁ → μ₂) (t : SubTerm L μ₁ n₁) :
+    (map fixed free t).val s e₂ ε₂ = t.val s (e₂ ∘ fixed) (ε₂ ∘ free) := val_bind _ _ _
 
 lemma val_subst (u : SubTerm L μ n) (t : SubTerm L μ (n + 1)) :
-    (subst u t).val S e Φ = t.val S (e <: u.val S e Φ) Φ :=
+    (subst u t).val s e ε = t.val s (e <: u.val s e ε) ε :=
   by simp[subst, val_bind]; congr; exact funext $ Fin.lastCases (by simp) (by simp)
 
-@[simp] lemma val_fixedSucc (a : S) (t : SubTerm L μ n) :
-    t.fixedSucc.val S (a :> e) Φ = t.val S e Φ := by simp[fixedSucc, val_map]
+@[simp] lemma val_fixedSucc (a : M) (t : SubTerm L μ n) :
+    t.fixedSucc.val s (a :> e) ε = t.val s e ε := by simp[fixedSucc, val_map, Function.comp]
+
+section onStructure₁
+variable (Φ : L₁ →ᵥ L₂) (s : Structure₁ L₂ M) (e : Fin n → M) (ε : μ → M)
+
+lemma val_onSubTerm {t : SubTerm L₁ μ n} :
+    val s e ε (Φ.onSubTerm t) = val (Φ.onStructure₁ s) e ε t :=
+  by induction t <;> simp[*, val!, Function.comp]
+
+end onStructure₁
 
 section Syntactic
-variable (Ψ : ℕ → S)
+variable (ε : ℕ → M)
 
 lemma val_shift (t : SyntacticSubTerm L n) :
-    t.shift.val S e Ψ = t.val S e (fun x => Ψ $ x + 1) := by simp[shift, val_map]
+    t.shift.val s e ε = t.val s e (ε ∘ Nat.succ) := by simp[shift, val_map]
 
-lemma val_free (a : S) (t : SyntacticSubTerm L (n + 1)) :
-    t.free.val S e (a :>ₙ Ψ) = t.val S (e <: a) Ψ :=
+lemma val_free (a : M) (t : SyntacticSubTerm L (n + 1)) :
+    t.free.val s e (a :>ₙ ε) = t.val s (e <: a) ε :=
   by simp[free, val_bind]; congr; exact funext $ Fin.lastCases (by simp) (by simp)
 
-lemma val_fix (a : S) (t : SyntacticSubTerm L n) :
-    t.fix.val S (e <: a) Ψ = t.val S e (a :>ₙ Ψ) :=
-  by simp[fix, val_bind]; congr; exact funext (Nat.cases (by simp) (by simp))
+lemma val_fix (a : M) (t : SyntacticSubTerm L n) :
+    t.fix.val s (e <: a) ε = t.val s e (a :>ₙ ε) :=
+  by simp[fix, val_bind, Function.comp]; congr; exact funext (Nat.cases (by simp) (by simp))
 
 end Syntactic
 
